$$ {t'=n}
D_n=D_0 \exp(-\frac{E}{{\rm R}T_{n-1}}) | (T_{n-1} \rightarrow D_n)\\
M_n=\frac{D_nc_{n-1}(1-c_{n-1})}{{\rm R}T_{n-1}} | (T_{n-1}, c_{n-1}, D_n \rightarrow M_n)\\
\mu_n=L(1-2c_{n-1})+{\rm R}T_{n-1}\ln \frac{c_{n-1}}{1-c_{n-1}}-2\kappa \nabla^2c_{n-1} | (T_{n-1}, c_{n-1} \rightarrow \mu_n)\\
\frac{\partial c_n}{\partial t}=\nabla \cdot (M_n \nabla \mu_n) | (M_n,\mu_n \rightarrow c_n)\\
\nabla \cdot (\sigma_{n-1} \nabla V_n)=0 | (\sigma_{n-1} \rightarrow V_n)\\
E_n=|\bold E|=|\nabla V_n| | (V_n \rightarrow E_n)\\
\Delta T_n=\frac{\sigma_{n-1}E_n^2t}{\rho C_{\rm P}} | (\sigma_{n-1},E_n \rightarrow \Delta T_n)\\
T_{n+1}=T_n+\Delta T_n | (T_n,\Delta T_n \rightarrow T_{n+1})\\
\frac{\partial T}{\partial t}=\alpha \nabla^2T \\
\frac{\partial \rho (\bold r)}{\partial t}=-\nabla \cdot \bold I = \nabla \cdot \{ \sigma (\bold r) \nabla V \} + s(\bold r) \\
V(\bold r) = \int_{\bold k} V(\bold k) \exp (i \bold k \cdot \bold r) \frac{d\bold k}{(2\pi)^3} \\
- \sigma_0 (k_1^2+k_2^2+k_3^2) V(\bold k) = -s(\bold k) - (ik_m) \left\{ \Delta \sigma (\bold r) \frac{\partial V}{\partial x_m} \right\}_{\bold k} \\

$$
